WIP

code/experimental/SPARKLE/dist/Hacl_Impl_Sparkle.c
@@ -28,7 +28,27 @@ uint32_t Hacl_Impl_Sparkle_size_word = (uint32_t)4U;
 
 uint32_t Hacl_Impl_Sparkle_vsize_rcon = (uint32_t)8U;
 
-const uint32_t *Hacl_Impl_Sparkle_rcon_buffer;
+const uint32_t *Hacl_Impl_Sparkle_rcon;
+
+void Hacl_Impl_Sparkle_arx(uint32_t c, uint32_t *b)
+{
+  uint32_t x = b[0U];
+  uint32_t y = b[1U];
+  uint32_t x1 = x + (y >> (uint32_t)31U | y << (uint32_t)1U);
+  uint32_t y1 = y ^ (x1 >> (uint32_t)24U | x1 << (uint32_t)8U);
+  uint32_t x2 = x1 ^ c;
+  uint32_t x3 = x2 + (y1 >> (uint32_t)17U | y1 << (uint32_t)15U);
+  uint32_t y2 = y1 ^ (x3 >> (uint32_t)17U | x3 << (uint32_t)15U);
+  uint32_t x4 = x3 ^ c;
+  uint32_t x5 = x4 + y2;
+  uint32_t y3 = y2 ^ (x5 >> (uint32_t)31U | x5 << (uint32_t)1U);
+  uint32_t x6 = x5 ^ c;
+  uint32_t x7 = x6 + (y3 >> (uint32_t)24U | y3 << (uint32_t)8U);
+  uint32_t y4 = y3 ^ (x7 >> (uint32_t)16U | x7 << (uint32_t)16U);
+  uint32_t x8 = x7 ^ c;
+  b[0U] = x8;
+  b[1U] = y4;
+}
 
 void Hacl_Impl_Sparkle_xor(uint32_t l, uint32_t *b, uint32_t *tx, uint32_t *ty)
 {
@@ -91,8 +111,89 @@ void Hacl_Impl_Sparkle_l_step(uint32_t n, uint32_t *perm, uint32_t i, uint32_t *
   rightBranch[(uint32_t)2U * index + (uint32_t)1U] = y;
 }
 
+void Hacl_Impl_Sparkle_l(uint32_t n, uint32_t *b)
+{
+  uint32_t *leftBranch = b;
+  uint32_t *rightBranch = b + n;
+  uint32_t index = n >> (uint32_t)1U;
+  Hacl_Impl_Sparkle_m(index, leftBranch);
+  for (uint32_t i = (uint32_t)0U; i < n >> (uint32_t)1U; i++)
+  {
+    Hacl_Impl_Sparkle_l_step(n >> (uint32_t)1U, rightBranch, i, (uint32_t *)(void *)(uint8_t)0U);
+  }
+}
+
+void Hacl_Impl_Sparkle_add2(uint32_t n, uint32_t i, uint32_t *b)
+{
+  uint32_t x0 = b[0U];
+  uint32_t y0 = b[1U];
+  uint32_t x1 = b[1U];
+  uint32_t y1 = b[2U];
+  uint32_t i1 = i & (uint32_t)7U;
+  uint32_t y01 = y0 ^ Hacl_Impl_Sparkle_rcon[i1];
+  uint32_t y11 = y1 ^ i1;
+  b[(uint32_t)2U * (uint32_t)0U] = x0;
+  b[(uint32_t)2U * (uint32_t)0U + (uint32_t)1U] = y01;
+  b[(uint32_t)2U * (uint32_t)1U] = x1;
+  b[(uint32_t)2U * (uint32_t)1U + (uint32_t)1U] = y11;
+}
+
+void Hacl_Impl_Sparkle_toBranch(uint32_t n, uint8_t *i, uint32_t *o)
+{
+  for (uint32_t i0 = (uint32_t)0U; i0 < (uint32_t)2U * n; i0++)
+  {
+    uint32_t *os = o;
+    uint8_t *bj = i + i0 * (uint32_t)4U;
+    uint32_t u = load32_le(bj);
+    uint32_t r = u;
+    uint32_t x = r;
+    os[i0] = x;
+  }
+}
+
+void Hacl_Impl_Sparkle_fromBranch(uint32_t n, uint32_t *i, uint8_t *o)
+{
+  for (uint32_t i0 = (uint32_t)0U; i0 < n * (uint32_t)2U; i0++)
+  {
+    store32_le(o + i0 * (uint32_t)4U, i[i0]);
+  }
+}
+
+void Hacl_Impl_Sparkle_arx_n_step(uint32_t n, uint32_t i, uint32_t *b)
+{
+  uint32_t *branchI = b + (uint32_t)2U * (n - (uint32_t)1U);
+  uint32_t rcon_i = Hacl_Impl_Sparkle_rcon[i];
+  Hacl_Impl_Sparkle_arx(rcon_i, branchI);
+}
+
+void Hacl_Impl_Sparkle_arx_n(uint32_t n, uint32_t *b)
+{
+  for (uint32_t i = (uint32_t)0U; i < n; i++)
+  {
+    Hacl_Impl_Sparkle_arx_n_step(n, i, b);
+  }
+}
+
+void Hacl_Impl_Sparkle_mainLoop_step(uint32_t n, uint32_t i, uint32_t *b)
+{
+  Hacl_Impl_Sparkle_add2(n, i, b);
+  Hacl_Impl_Sparkle_arx_n(n, b);
+  Hacl_Impl_Sparkle_l(n, b);
+}
+
+void Hacl_Impl_Sparkle_mainLoop(uint32_t n, uint32_t *b, uint32_t steps)
+{
+  for (uint32_t i = (uint32_t)0U; i < steps; i++)
+  {
+    Hacl_Impl_Sparkle_mainLoop_step(n, i, b);
+  }
+}
+
 void Hacl_Impl_Sparkle_sparkle256(uint32_t steps, uint8_t *i, uint8_t *o)
 {
-  
+  uint32_t temp[4U] = { 0U };
+  Hacl_Impl_Sparkle_toBranch((uint32_t)(krml_checked_int_t)4, i, temp);
+  Hacl_Impl_Sparkle_mainLoop((uint32_t)(krml_checked_int_t)4, temp, steps);
+  Hacl_Impl_Sparkle_fromBranch((uint32_t)(krml_checked_int_t)4, (uint32_t *)steps, o);
 }
 
