code/experimental/SPARKLE/Hacl.Impl.Sparkle.fst
@@ -20,7 +20,7 @@ let vsize_rcon: size_t = 8ul
 
 
 inline_for_extraction
-let rcon_buffer: x: glbuffer uint32 vsize_rcon 
+let rcon: x: glbuffer uint32 vsize_rcon 
   {witnessed #uint32 #vsize_rcon x (Lib.Sequence.of_list rcon_list) /\ recallable x} =
   createL_global rcon_list
 
@@ -31,10 +31,9 @@ inline_for_extraction
 type branch branch_len = lbuffer uint32 (2ul *! branch_len)
 
 
-inline_for_extraction noextract
-val arx: uint32 -> branch1: branch 1ul -> Stack unit 
-  (requires fun h -> live h branch1)
-  (ensures fun h0 _ h1 -> modifies (loc branch1) h0 h1)
+val arx: uint32 -> b: branch 1ul -> Stack unit 
+  (requires fun h -> live h b)
+  (ensures fun h0 _ h1 -> True)
     
 let arx c b = 
   let x, y = index b (size 0), index b (size 1) in 
@@ -58,13 +57,14 @@ let arx c b =
   upd b (size 0) x;
   upd b (size 1) y
 
+
 inline_for_extraction noextract
 val l1: x:uint32 -> Tot uint32
 let l1 x = (x <<<. size 16)  ^. (x &. (u32 0xffff))
 
 
 inline_for_extraction noextract
-val getBranch: #l: branch_len -> b: branch l -> i: size_t {v i < v l / 2} -> 
+val getBranch: #l: branch_len -> b: branch l -> i: size_t {v i <= v l / 2} -> 
   Stack (tuple2 uint32 uint32)
   (requires fun h -> live h b)
   (ensures fun h0 _ h1 -> modifies0 h0 h1)
@@ -73,7 +73,7 @@ let getBranch #l b i =  Lib.Buffer.index b i, Lib.Buffer.index b (i +! 1ul)
 
 
 inline_for_extraction noextract 
-val setBranch: #n: branch_len -> i: size_t {v i < v n / 2} -> branch1 -> b: branch n -> 
+val setBranch: #n: branch_len -> i: size_t {v i <= v n / 2} -> branch1 -> b: branch n -> 
   Stack unit 
   (requires fun h -> live h b)
   (ensures fun h0 _ h1 -> modifies (loc b) h0 h1)  
@@ -87,7 +87,7 @@ inline_for_extraction noextract
 val xor_step: #l: branch_len -> b: branch l
   -> tx: lbuffer uint32 (size 1) 
   -> ty: lbuffer uint32 (size 1) 
-   -> i: size_t {v i < v l / 2} ->
+   -> i: size_t {v i <= v l / 2} ->
   Stack unit
     (requires fun h -> live h b /\ live h tx /\ live h ty /\ disjoint tx ty)
     (ensures fun h0 _ h1 -> modifies (loc tx |+| loc ty) h0 h1)
@@ -100,7 +100,7 @@ let xor_step #l b tx ty i =
   upd tx (size 0) (yi ^. ty_0)
 
 
-val xor: #l: branch_len {v l % 2 == 0} -> b: branch l-> tx: lbuffer uint32 (size 1) -> ty: lbuffer uint32 (size 1) ->  
+val xor: #l: branch_len -> b: branch l-> tx: lbuffer uint32 (size 1) -> ty: lbuffer uint32 (size 1) ->  
   Stack unit
     (requires fun h -> live h b /\ live h ty /\ live h tx /\ disjoint tx ty)
     (ensures fun h0 _ h1 -> modifies (loc tx |+| loc ty) h0 h1)
@@ -108,12 +108,12 @@ val xor: #l: branch_len {v l % 2 == 0} -> b: branch l-> tx: lbuffer uint32 (size
 let xor #l b tx ty = 
   let h0 = ST.get() in 
   Lib.Loops.for 0ul (l >>. 1ul) 
-    (fun h i ->live h b /\ live h ty /\ live h tx /\ disjoint tx ty /\ modifies (loc tx |+| loc ty) h0 h) 
-    (fun (i: size_t {v i < v l / 2}) -> xor_step b tx ty i)
+    (fun h i -> live h b /\ live h ty /\ live h tx /\ disjoint tx ty /\ modifies (loc tx |+| loc ty) h0 h) 
+    (fun (i: size_t {v i <= v l / 2}) -> xor_step b tx ty i)
     
 
 inline_for_extraction noextract
-val xor_x_step: #l: branch_len -> b: branch l -> lty: uint32 -> ltx: uint32 -> i: size_t {v i < v l / 2} -> 
+val xor_x_step: #l: branch_len -> b: branch l -> lty: uint32 -> ltx: uint32 -> i: size_t {v i <= v l / 2} -> 
   Stack unit 
     (requires fun h -> live h b)
     (ensures fun h0 _ h1 -> modifies (loc b) h0 h1)
@@ -133,10 +133,10 @@ let xor_x #l b lty ltx =
   let h0 = ST.get() in 
   Lib.Loops.for (0ul) (l >>. 1ul)  
     (fun h i -> live h b /\ modifies (loc b) h0 h) 
-    (fun (i: size_t {v i < v l / 2})  -> xor_x_step b lty ltx i)
+    (fun (i: size_t {v i <= v l / 2}) -> xor_x_step b lty ltx i)
 
 
-val m: #l: branch_len {v l % 2 == 0} -> b: branch l -> Stack unit 
+val m: #l: branch_len -> b: branch l -> Stack unit 
   (requires fun h -> live h b)
   (ensures fun h0 _ h1 -> modifies (loc b) h0 h1)
 
@@ -144,15 +144,15 @@ let m #n b =
   push_frame();
     let tx = create (size 1) (u32 0) in 
     let ty = create (size 1) (u32 0) in 
-  xor #n b tx ty;
-  let ltx = l1 (index tx (size 0)) in
-  let lty = l1 (index ty (size 0)) in 
-  xor_x #n b lty ltx;
+    
+    xor #n b tx ty;
+    let ltx = l1 (index tx (size 0)) in
+    let lty = l1 (index ty (size 0)) in 
+    xor_x #n b lty ltx;
   pop_frame()
 
 
-
-val l_step: (#n: branch_len) -> (perm: branch n) -> i: size_t {v i < v n / 2} -> (rightBranch : branch n) -> Stack unit 
+val l_step: #n: branch_len -> perm: branch n -> i: size_t {v i <= v n / 2} -> (rightBranch : branch n) -> Stack unit 
   (requires fun h -> live h perm /\ live h rightBranch)
   (ensures fun h0 _ h1 -> modifies (loc rightBranch) h0 h1)
 
@@ -162,9 +162,110 @@ let l_step #n perm i rightBranch =
   let branchIUpd = xi ^. p0i, yi ^. p1i in
   
   let index = rotate_right n 1ul in 
-  setBranch #n index branchIUpd rightBranch;
   
-  admit()
+  assume (v index  <= v n / 2);
+  
+  setBranch #n index branchIUpd rightBranch
+
+
+val l: #n: branch_len {v n % 2 == 0} -> b: branch n -> Stack unit 
+  (requires fun h -> live h b)
+  (ensures fun h0 _ h1 -> modifies (loc b) h0 h1)
+
+let l #n b = 
+  let leftBranch = sub b (size 0) n in 
+  let rightBranch = sub b n n in 
+
+  let index : branch_len = (n >>. 1ul) in 
+  let perm = m #index leftBranch in 
+
+ (* assume (v (n >>. 1ul) == v n /  *)
+  Lib.Loops.for 0ul (n >>. 1ul) 
+  (fun h i -> live h b)
+  (fun (i: size_t {v i <= v n / 2}) -> l_step #(n >>. 1ul) rightBranch i perm)
+
+
+
+val add2: #n: branch_len {v n >= 4} -> i: size_t -> b:branch n -> Stack unit 
+  (requires fun h -> live h b) 
+  (ensures fun h0 _ h1 -> modifies (loc b) h0 h1)
+
+let add2 #n i b = 
+  let (x0, y0) = getBranch #n b (size 0) in 
+  recall_contents rcon (Lib.Sequence.of_list rcon_list); 
+  let (x1,y1) =  getBranch #n b (size 1) in 
+
+  (* let y0 = y0 ^. index rcon (size (i % vsize_rcon)) in *)  
+  let i0 = logand i (size 7) in 
+    logand_mask i (size 7) 3; 
+  let y0 = y0 ^. index rcon i0 in
+  let y1 = y1 ^. (to_u32 i0) in
+  setBranch (size 0) (x0, y0) b;
+  setBranch #n (size 1) (x1, y1) b
+
+
+val toBranch: #n: branch_len -> i: lbuffer uint8 (size 8 *! n) -> o: branch n -> 
+  Stack unit 
+  (requires fun h -> True)
+  (ensures fun h0 _ h1 -> True)
+
+let toBranch #n i o = 
+  uints_from_bytes_le o i 
+
+
+val fromBranch: #n: branch_len -> i: branch n -> o: lbuffer uint8 (size 8 *! n) -> 
+  Stack unit 
+  (requires fun h -> True)
+  (ensures fun h0 _ h1 -> True)
+
+let fromBranch #n i o = 
+  uints_to_bytes_le (n *! 2ul) o i
+
+
+val arx_n_step: #n: branch_len -> i: size_t {v i < v n / 2} -> b: branch n -> 
+  Stack unit 
+  (requires fun h -> live h b)
+  (ensures fun h0 _ h1 -> True)
+
+let arx_n_step #n i b = 
+  let branchI = sub b (size 2 *! (n -. 1ul)) (size 2) in 
+    recall_contents rcon (Lib.Sequence.of_list rcon_list); 
+  let rcon_i = index rcon i in 
+  arx rcon_i branchI
+
+
+val arx_n: #n: branch_len -> branch n -> 
+  Stack unit 
+  (requires fun h -> True)
+  (ensures fun h0 _ h1 -> True)
+
+let arx_n #n b =
+  Lib.Loops.for 0ul n
+  (fun h i -> live h b)
+  (fun (i: size_t {v i < v n / 2}) -> arx_n_step i b)
+
+
+val mainLoop_step: #n: branch_len {v n >= 4 /\ v n % 2 == 0 } ->  i: size_t -> branch n ->
+  Stack unit 
+  (requires fun h -> True)
+  (ensures fun h0 _ h1 -> True)
+
+
+let mainLoop_step #n i b = 
+  add2 i b;
+  arx_n #n b;
+  l #n b
+
+
+val mainLoop: #n: branch_len {n >= 2 /\ n % 2 == 0} -> b: branch n -> steps: size_t -> 
+  Stack unit 
+  (requires fun h -> True)
+  (ensures fun h0 _ h1 -> True)
+
+let mainLoop #n b steps = 
+  Lib.Loops.for 0ul steps
+  (fun h i -> live h b)
+  (fun (i: size_t {v i < v n / 2}) -> mainLoop_step i b)
 
 
 val sparkle256: steps: size_t -> i: lbuffer (uint8) (size 32) -> o: lbuffer (uint8) (size 32) ->
@@ -172,4 +273,10 @@ val sparkle256: steps: size_t -> i: lbuffer (uint8) (size 32) -> o: lbuffer (uin
   (requires fun h -> True)
   (ensures fun h0 _ h1 -> True)
 
-let sparkle256 steps i o = ()
+let sparkle256 steps i o =
+  push_frame();
+    let temp = create (size 4) (u32 0) in 
+    toBranch #4 i temp;
+    mainLoop #4 temp steps;
+    fromBranch #4 steps o; 
+  pop_frame()
